tests/lean/run/subst_heq.lean
@@ -1,0 +1,4 @@
+example (a b : nat) (h : a == b) : a + 1 = b + 1 :=
+begin
+  subst h
+end
